BPlusTree_Set.thy
@@ -882,7 +882,7 @@ lemma height_up\<^sub>i_merge: "height_up\<^sub>i (Up\<^sub>i l a r) = height t 
 lemma ins_height: "height_up\<^sub>i (ins k x t) = height t"
 proof(induction k x t rule: ins.induct)
   case (2 k x ts t)
-  then obtain ls rs where split: "split ts x = (ls,rs)"
+  then obtain ls rs where split_list: "split ts x = (ls,rs)"
     by (meson surj_pair)
   then have split_append: "ts = ls@rs"
     using split_conc
@@ -891,7 +891,7 @@ proof(induction k x t rule: ins.induct)
   proof (cases rs)
     case Nil
     then have height_sub: "height_up\<^sub>i (ins k x t) = height t"
-      using 2 by (simp add: split)
+      using 2 by (simp add: split_list)
     then show ?thesis
     proof (cases "ins k x t")
       case (T\<^sub>i a)
@@ -899,13 +899,13 @@ proof(induction k x t rule: ins.induct)
         using height_sub
         by simp
       then show ?thesis
-        using T\<^sub>i Nil split split_append
+        using T\<^sub>i Nil split_list split_append
         by simp
     next
       case (Up\<^sub>i l a r)
       then have "height (Node ls t) = height (Node (ls@[(l,a)]) r)"
         using height_bplustree_order height_sub by (induction ls) auto
-      then show ?thesis using 2 Nil split Up\<^sub>i split_append
+      then show ?thesis using 2 Nil split_list Up\<^sub>i split_append
         by (simp del: node\<^sub>i.simps add: node\<^sub>i_height)
     qed
   next
@@ -913,7 +913,7 @@ proof(induction k x t rule: ins.induct)
     then obtain sub sep where a_split: "a = (sub,sep)"
       by (cases a) auto
     then have height_sub: "height_up\<^sub>i (ins k x sub) = height sub"
-      by (metis "2.IH"(2) a_split Cons split)
+      by (metis "2.IH"(2) a_split Cons split_list)
     then show ?thesis
     proof (cases "ins k x sub")
       case (T\<^sub>i a)
@@ -922,7 +922,7 @@ proof(induction k x t rule: ins.induct)
       then have "height (Node (ls@(sub,sep)#rs) t) = height (Node (ls@(a,sep)#rs) t)"
         by auto
       then show ?thesis 
-        using T\<^sub>i height_sub Cons 2 split a_split split_append
+        using T\<^sub>i height_sub Cons 2 split_list a_split split_append
         by (auto simp add: image_Un max.commute finite_set_ins_swap)
     next
       case (Up\<^sub>i l a r)
@@ -930,7 +930,7 @@ proof(induction k x t rule: ins.induct)
         using height_up\<^sub>i_merge height_sub
         by fastforce
       then show ?thesis
-        using Up\<^sub>i Cons 2 split a_split split_append
+        using Up\<^sub>i Cons 2 split_list a_split split_append
         by (auto simp del: node\<^sub>i.simps simp add: node\<^sub>i_height image_Un max.commute finite_set_ins_swap)
     qed
   qed
@@ -2130,12 +2130,12 @@ lemma node\<^sub>i_bal_up\<^sub>i:
   using assms
 proof(cases "length ts \<le> 2*k")
   case False
-  then obtain ls sub sep rs where split: "split_half ts = (ls@[(sub,sep)], rs)"
+  then obtain ls sub sep rs where split_list: "split_half ts = (ls@[(sub,sep)], rs)"
     using node\<^sub>i_cases by blast
   then have "node\<^sub>i k ts t = Up\<^sub>i (Node ls sub) sep (Node rs t)"
     using False by auto
   moreover have "ts = ls@(sub,sep)#rs"
-    by (metis append_Cons append_Nil2 append_eq_append_conv2 local.split same_append_eq split_half_conc)
+    by (metis append_Cons append_Nil2 append_eq_append_conv2 local.split_list same_append_eq split_half_conc)
   ultimately show ?thesis
     using bal_list_merge[of ls sub sep rs t] assms
     by (simp del: bal.simps bal_up\<^sub>i.simps)
@@ -3522,64 +3522,64 @@ lemma isin_sorted: "sorted_less (xs@a#ys) \<Longrightarrow>
   by (auto simp: isin_simps2)
 
 locale split_list =
-  fixes split ::  "('a::{linorder,order_top}) list \<Rightarrow> 'a \<Rightarrow> 'a list \<times> 'a list"
-  assumes split_req:
-    "\<lbrakk>split ks p = (kls,krs)\<rbrakk> \<Longrightarrow> ks = kls @ krs"
-    "\<lbrakk>split ks p = (kls@[sep],krs); sorted_less ks\<rbrakk> \<Longrightarrow> sep < p"
-    "\<lbrakk>split ks p = (kls,(sep)#krs); sorted_less ks\<rbrakk> \<Longrightarrow> p \<le> sep"
+  fixes split_list ::  "('a::{linorder,order_top}) list \<Rightarrow> 'a \<Rightarrow> 'a list \<times> 'a list"
+  assumes split_list_req:
+    "\<lbrakk>split_list ks p = (kls,krs)\<rbrakk> \<Longrightarrow> ks = kls @ krs"
+    "\<lbrakk>split_list ks p = (kls@[sep],krs); sorted_less ks\<rbrakk> \<Longrightarrow> sep < p"
+    "\<lbrakk>split_list ks p = (kls,(sep)#krs); sorted_less ks\<rbrakk> \<Longrightarrow> p \<le> sep"
 begin
 
 fun isin_list :: "'a \<Rightarrow> 'a list \<Rightarrow> bool" where
-  "isin_list x ks = (case split ks x of 
+  "isin_list x ks = (case split_list ks x of 
     (ls,Nil) \<Rightarrow> False |
     (ls,sep#rs) \<Rightarrow> sep = x
 )"
 
 fun insert_list where
-  "insert_list x ks = (case split ks x of 
+  "insert_list x ks = (case split_list ks x of 
     (ls,Nil) \<Rightarrow> ls@[x] |
     (ls,sep#rs) \<Rightarrow> if sep = x then ks else ls@x#sep#rs
 )"
 
 fun delete_list where
-  "delete_list x ks = (case split ks x of 
+  "delete_list x ks = (case split_list ks x of 
     (ls,Nil) \<Rightarrow> ks |
     (ls,sep#rs) \<Rightarrow> if sep = x then ls@rs else ks
 )"
 
-lemmas split_conc = split_req(1)
-lemmas split_sorted = split_req(2,3)
+lemmas split_list_conc = split_list_req(1)
+lemmas split_list_sorted = split_list_req(2,3)
 
 
 (* lift to split *)
 
-lemma isin_sorted_split:
+lemma isin_sorted_split_list:
 assumes "sorted_less xs"
-    and "split xs x = (ls, rs)"
+    and "split_list xs x = (ls, rs)"
   shows "(x \<in> set xs) = (x \<in> set rs)"
 proof (cases ls)
   case Nil
   then have "xs = rs"
-    using assms by (auto dest!: split_conc)
+    using assms by (auto dest!: split_list_conc)
   then show ?thesis by simp
 next
   case Cons
   then obtain ls' sep where ls_tail_split: "ls = ls' @ [sep]"
     by (metis list.simps(3) rev_exhaust)
   then have x_sm_sep: "sep < x"
-    using split_req(2)[of xs x ls' sep rs]
+    using split_list_req(2)[of xs x ls' sep rs]
     using assms sorted_cons sorted_snoc 
     by blast
   moreover have "xs = ls@rs"
-    using assms split_conc by simp
+    using assms split_list_conc by simp
   ultimately show ?thesis
     using isin_sorted[of ls' sep rs]
     using assms ls_tail_split
     by auto
 qed
 
-lemma isin_sorted_split_right:
-  assumes "split ts x = (ls, sep#rs)"
+lemma isin_sorted_split_list_right:
+  assumes "split_list ts x = (ls, sep#rs)"
     and "sorted_less ts"
   shows "x \<in> set (sep#rs) = (x = sep)"
 proof (cases rs)
@@ -3589,9 +3589,9 @@ proof (cases rs)
 next
   case (Cons sep' rs)
   from assms have "x < sep'"
-    by (metis le_less less_trans list.set_intros(1) local.Cons sorted_Cons_iff sorted_wrt_append split_conc split_sorted(2))
+    by (metis le_less less_trans list.set_intros(1) local.Cons sorted_Cons_iff sorted_wrt_append split_list_conc split_list_sorted(2))
   moreover have "ts = ls@sep#sep'#rs"
-    using split_conc[OF assms(1)] Cons by auto
+    using split_list_conc[OF assms(1)] Cons by auto
   moreover have "sorted_less (sep#sep'#rs)" 
     using Cons assms calculation(2) sorted_wrt_append by blast
   ultimately show ?thesis
@@ -3604,18 +3604,18 @@ theorem isin_list_set:
   assumes "sorted_less xs"
   shows "isin_list x xs = (x \<in> set xs)"
   using assms
-  using isin_sorted_split[of xs x]
-  using isin_sorted_split_right[of xs x]
+  using isin_sorted_split_list[of xs x]
+  using isin_sorted_split_list_right[of xs x]
   by (auto split!: list.splits)
 
-lemma insert_sorted_split:
+lemma insert_sorted_split_list:
 assumes "sorted_less xs"
-    and "split xs x = (ls, rs)"
+    and "split_list xs x = (ls, rs)"
   shows "ins_list x xs = ls @ ins_list x rs"
 proof (cases ls)
   case Nil
   then have "xs = rs"
-    using assms by (auto dest!: split_conc)
+    using assms by (auto dest!: split_list_conc)
   then show ?thesis 
     using Nil by simp
 next
@@ -3623,25 +3623,25 @@ next
   then obtain ls' sep where ls_tail_split: "ls = ls' @ [sep]"
     by (metis list.simps(3) rev_exhaust)
   then have x_sm_sep: "sep < x"
-    using split_req(2)[of xs x ls' sep rs]
+    using split_list_req(2)[of xs x ls' sep rs]
     using assms sorted_cons sorted_snoc 
     by blast
   moreover have "xs = ls@rs"
-    using assms split_conc by simp
+    using assms split_list_conc by simp
   ultimately show ?thesis
     using ins_list_sorted[of ls' sep x rs]
     using assms ls_tail_split sorted_wrt_append[of "(<)" ls rs]
     by auto
 qed
 
-lemma insert_sorted_split_right:
-  assumes "split ts x = (ls, sep#rs)"
+lemma insert_sorted_split_list_right:
+  assumes "split_list ts x = (ls, sep#rs)"
     and "sorted_less ts"
     and "x \<noteq> sep"
   shows "ins_list x (sep#rs) = (x#sep#rs)"
 proof -
   have "x < sep"
-    by (meson assms(1) assms(2) assms(3) le_neq_trans split_sorted(2))
+    by (meson assms(1) assms(2) assms(3) le_neq_trans split_list_sorted(2))
   then show ?thesis
     using ins_list_sorted[of "[]" sep]
     using assms
@@ -3652,19 +3652,19 @@ qed
 theorem insert_list_set: 
   assumes "sorted_less xs"
   shows "insert_list x xs = ins_list x xs"
-  using assms split_conc
-  using insert_sorted_split[of xs x]
-  using insert_sorted_split_right[of xs x]
+  using assms split_list_conc
+  using insert_sorted_split_list[of xs x]
+  using insert_sorted_split_list_right[of xs x]
   by (auto split!: list.splits prod.splits)
 
-lemma delete_sorted_split:
+lemma delete_sorted_list_split:
 assumes "sorted_less xs"
-    and "split xs x = (ls, rs)"
+    and "split_list xs x = (ls, rs)"
   shows "del_list x xs = ls @ del_list x rs"
 proof (cases ls)
   case Nil
   then have "xs = rs"
-    using assms by (auto dest!: split_conc)
+    using assms by (auto dest!: split_list_conc)
   then show ?thesis 
     using Nil by simp
 next
@@ -3672,27 +3672,27 @@ next
   then obtain ls' sep where ls_tail_split: "ls = ls' @ [sep]"
     by (metis list.simps(3) rev_exhaust)
   then have x_sm_sep: "sep < x"
-    using split_req(2)[of xs x ls' sep rs]
+    using split_list_req(2)[of xs x ls' sep rs]
     using assms sorted_cons sorted_snoc 
     by blast
   moreover have "xs = ls@rs"
-    using assms split_conc by simp
+    using assms split_list_conc by simp
   ultimately show ?thesis
     using del_list_sorted[of ls' sep rs]
     using assms ls_tail_split sorted_wrt_append[of "(<)" ls rs]
     by auto
 qed
 
-lemma delete_sorted_split_right:
-  assumes "split ts x = (ls, sep#rs)"
+lemma delete_sorted_split_list_right:
+  assumes "split_list ts x = (ls, sep#rs)"
     and "sorted_less ts"
     and "x \<noteq> sep"
   shows "del_list x (sep#rs) = sep#rs"
 proof -
   have "sorted_less (sep#rs)"
-    by (metis assms(1) assms(2) sorted_wrt_append split_list.split_conc split_list_axioms)
+    by (metis assms(1) assms(2) sorted_wrt_append split_list.split_list_conc split_list_axioms)
   moreover have "x < sep"
-    by (meson assms(1) assms(2) assms(3) le_neq_trans split_sorted(2))
+    by (meson assms(1) assms(2) assms(3) le_neq_trans split_list_sorted(2))
   ultimately show ?thesis
     using del_list_sorted[of "[]" sep rs x]
     by simp
@@ -3702,9 +3702,9 @@ qed
 theorem delete_list_set: 
   assumes "sorted_less xs"
   shows "delete_list x xs = del_list x xs"
-  using assms split_conc[of xs x]
-  using delete_sorted_split[of xs x]
-  using delete_sorted_split_right[of xs x]
+  using assms split_list_conc[of xs x]
+  using delete_sorted_split_list[of xs x]
+  using delete_sorted_split_list_right[of xs x]
   by (auto split!: list.splits prod.splits)
 
 end
@@ -3721,5 +3721,7 @@ begin
 sublocale split split isin_list insert_list delete_list 
   using isin_list_set insert_list_set delete_list_set
   by unfold_locales auto
+
+end
 
 end
